BoogieLang/Semantics.thy
@@ -474,12 +474,23 @@ inductive red_expr :: "'a absval_ty_fun \<Rightarrow> var_context \<Rightarrow> 
 inductive_cases RedBinOp_case[elim!]: "A,\<Lambda>,\<Gamma>,\<Omega> \<turnstile> \<langle>(e1 \<guillemotleft>bop\<guillemotright> e2), n_s\<rangle> \<Down> v"
 inductive_cases RedUnOp_case[elim!]: "A,\<Lambda>,\<Gamma>,\<Omega> \<turnstile> \<langle>UnOp uop e1, n_s\<rangle> \<Down> v"
 inductive_cases RedFunOp_case[elim!]: "A,\<Lambda>,\<Gamma>,\<Omega> \<turnstile> \<langle> FunExp f ty_args args, n_s \<rangle> \<Down> v"
+inductive_cases RedCondExp_case[elim!]: "A,\<Lambda>,\<Gamma>,\<Omega> \<turnstile> \<langle> CondExp cond thn els, n_s \<rangle> \<Down> v"
 inductive_cases RedOld_case[elim!]: "A,\<Lambda>,\<Gamma>,\<Omega> \<turnstile> \<langle>Old  e, n_s\<rangle> \<Down> v"
 inductive_cases RedLit_case[elim!]: "A,\<Lambda>,\<Gamma>,\<Omega> \<turnstile> \<langle>(Lit l), n_s\<rangle> \<Down> LitV l"
 inductive_cases RedVar_case[elim!]: "A,\<Lambda>,\<Gamma>,\<Omega> \<turnstile> \<langle>(Var x), n_s\<rangle> \<Down> v"
 inductive_cases RedBVar_case[elim!]: "A,\<Lambda>,\<Gamma>,\<Omega> \<turnstile> \<langle>(BVar i), n_s\<rangle> \<Down> v"
 inductive_cases RedForallTrue_case: "A,\<Lambda>,\<Gamma>,\<Omega> \<turnstile> \<langle>Forall ty e, n_s\<rangle> \<Down> LitV (LBool True)"
 inductive_cases RedForallFalse_case: "A,\<Lambda>,\<Gamma>,\<Omega> \<turnstile> \<langle>Forall ty e, n_s\<rangle> \<Down> LitV (LBool False)"
+
+lemma red_cond_exp_cases:
+  assumes "A,\<Lambda>,\<Gamma>,\<Omega> \<turnstile> \<langle>CondExp cond thn els, n_s \<rangle> \<Down> v"
+  obtains b
+  where "(A,\<Lambda>,\<Gamma>,\<Omega> \<turnstile> \<langle>cond, n_s\<rangle> \<Down> BoolV b) \<and> (A,\<Lambda>,\<Gamma>,\<Omega> \<turnstile> \<langle>if b then thn else els, n_s\<rangle> \<Down> v)"
+  using assms
+  apply cases
+   apply fastforce
+  apply fastforce
+  done
 
 definition expr_sat :: "'a absval_ty_fun \<Rightarrow> var_context \<Rightarrow> 'a fun_interp \<Rightarrow> rtype_env \<Rightarrow> 'a nstate \<Rightarrow> expr \<Rightarrow> bool"
   where "expr_sat A \<Lambda> \<Gamma> \<Omega> n_s e = (A,\<Lambda>,\<Gamma>,\<Omega> \<turnstile> \<langle>e, n_s\<rangle> \<Down> LitV (LBool True))"
